restrutucing

SATsolver/Experiment/DPLL/impl.lean
@@ -14,7 +14,7 @@ def internal (t : Trail)(f : Formula)(v : Variables)(vz : v ≠ 0)(wf : f.wf ∧
         exists a
       have com' : Completenes.inv (backtrack t bcwf twf.1) f := by
         simp at con
-        have := Completenes.from_con con
+        have := Completenes.con_no_exist con
         exact bck_completeness2 (twf := twf.1) (wf := bcwf) com this
       internal (backtrack t bcwf twf.1) f v vz wf (bck_preserves_twf (tf := twf.2)) com'
     else (false, t)
@@ -33,9 +33,9 @@ def internal (t : Trail)(f : Formula)(v : Variables)(vz : v ≠ 0)(wf : f.wf ∧
         simp only [copt] at h
         have := List.get_find?_mem h
         simp[c, copt, this]
-      have com' : Completenes.inv (propogate t c this) f := by
+      have com' : Completenes.inv (propagate t c this) f := by
         exact ppg_completeness2 twf wf.1 com cmem
-      internal (propogate t c this) f v vz wf (ppg_preserves_wf cmem (fwf := wf.1) (twf := twf)) com'
+      internal (propagate t c this) f v vz wf (ppg_preserves_wf cmem (fwf := wf.1) (twf := twf)) com'
     else
       have ud : t¿f := by
         simp at *
@@ -102,3 +102,130 @@ def DPLL(f : Formula)(v : Variables)(wf : f.wf ∧ v.wf f) :=
   match f with
   | [] => (true, [])
   | hd::tl => internal [] (hd::tl) v (Variables.f_cons_ne_zero wf.2 (fwf := wf.1)) wf (by simp[Trail.wf, Trail.names]) (by simp[Completenes.inv])
+
+
+def occurences(f : Formula)(v : Variables)(_ : f.wf ∧ v.wf f) : List (Nat × Nat):=
+  ((List.range v).map (fun n => ( n+1, f.names.count (n + 1) ))).mergeSort (fun (_,o₁) (_,o₂)=> o₁ >= o₂)
+
+theorem n_f_n_occ {n : Nat}{f : Formula}{v : Variables}(wf : f.wf ∧ v.wf f):
+  n ∈ f.names → ∃ o, (n, o) ∈ occurences f v wf := by
+  intro nin
+  have nzero : n ≠ 0 := by
+    have := Formula.zero_not_names wf.1
+    intro contra
+    rw[contra] at nin
+    contradiction
+  simp[occurences, Variables.wf, Formula.wf] at wf ⊢
+  have nlev := wf.2.1 n nin
+  let o : Nat := f.names.count n
+  let m : Nat := n -1
+  have : m + 1 = n := by
+    have : n > 0 := Nat.zero_lt_of_ne_zero nzero
+    simp[m, this, Nat.sub_one_add_one_eq_of_pos]
+  exists o, m
+  simp[this, o]
+  have mltn : m < n := by simp[←this]
+  exact Nat.lt_of_lt_of_le mltn nlev
+
+theorem nocc_nf{res : Nat × Nat}{f : Formula}{v : Variables}(wf : f.wf ∧ v.wf f):
+  res ∈ occurences f v wf → res.1 ∈ f.names := by
+  intro h
+  simp[occurences] at h
+  obtain ⟨ a, altv, ahen ⟩ := h
+  simp[Formula.wf, Variables.wf] at wf
+  have nlev : res.1 ≤ v := by
+    have := Nat.succ_le_of_lt altv
+    rw[← ahen, ←Nat.succ_eq_add_one]
+    exact this
+  have nnzero : res.1 ≠ 0 := by
+    simp[← ahen]
+  exact wf.2.2 res.1 nlev nnzero
+
+
+def internal_moma (t : Trail)(f : Formula)(v : Variables) (occ : List (Nat × Nat))(vz : v ≠ 0)(wf : f.wf ∧ v.wf f)(twf : t.wf ∧ ∀ n ∈ t.names, n ∈ f.names)(com : Completenes.inv t f)(hocc : occ = occurences f v wf): Bool × Trail :=
+  if sat : decide (t ⊨ f) then
+    (true, t)
+  else if con : decide (t ⊭ f) then
+    if anyDec : t.any ALit.decidedB then
+      have bcwf : ∃ a ∈ t, a.decidedP := by
+        simp[ALit.decidedP_iff_decidedB] at anyDec
+        obtain ⟨ a, amem, adec ⟩ := anyDec
+        exists a
+      have com' : Completenes.inv (backtrack t bcwf twf.1) f := by
+        simp at con
+        have := Completenes.con_no_exist con
+        exact bck_completeness2 (twf := twf.1) (wf := bcwf) com this
+      internal_moma (backtrack t bcwf twf.1) f v occ vz wf (bck_preserves_twf (tf := twf.2)) com' hocc
+    else (false, t)
+  else
+    let copt := f.find? (fun c => c.unit t)
+    if h : copt.isSome then
+      let c := copt.get h
+      have : c.unit t := by
+        have cunit : copt = some c := by
+          simp[c]
+        simp[copt] at cunit
+        have := List.find?_some cunit
+        simp at this
+        exact this
+      have cmem : c ∈ f := by
+        simp only [copt] at h
+        have := List.get_find?_mem h
+        simp[c, copt, this]
+      have com' : Completenes.inv (propagate t c this) f := by
+        exact ppg_completeness2 twf wf.1 com cmem
+      internal_moma (propagate t c this) f v occ vz wf (ppg_preserves_wf cmem (fwf := wf.1) (twf := twf)) com' hocc
+    else
+      have ud : t¿f := by
+        simp at *
+        exact Formula.nSatCon_ud sat con
+      have nexi := Formula.ud_exists_udname ud
+      let nopt := (occ.find? (fun (n,o) => n ∉ t.names))
+      have nsome : nopt.isSome := by
+        obtain ⟨ n, hn ⟩ := nexi
+        have := n_f_n_occ wf hn.1
+        simp[nopt, hocc]
+        exists n
+        simp[this, hn.2]
+      let res := nopt.get nsome
+      have : t ¿ (Lit.pos res.1) := by
+        simp[Undecided.ud]
+        have heq : nopt = some res := by simp[res]
+        simp[nopt] at heq
+        have := List.find?_some heq
+        simp[Lit.name] at ⊢ this
+        exact this
+      have lmem : (Lit.pos res.1).name ∈ f.names := by
+        have : res ∈ occ := by
+          simp[res, nopt, List.get_find?_mem]
+        simp[hocc] at this
+        have := nocc_nf wf this
+        simp[Lit.name]
+        exact this
+      have com' : Completenes.inv (dec (Lit.pos res.1) t this) f := by
+        exact dec_preserves_completenes lmem com
+      internal_moma (dec (Lit.pos res.1) t this) f v occ vz wf (dec_preserves_wf (fwf := wf.1) (twf := twf) lmem) com' hocc
+termination_by distance t v vz
+decreasing_by
+  have : t.length ≤ v := Trail.mem_vwf twf.1 twf.2 wf.2
+  exact distance_bc this
+  have : t.length < v := by
+    simp at sat con
+    have := Trail.ud_vars twf.1 wf.1 wf.2 twf.2 (Formula.nSatCon_ud sat con)
+    simp[Trail.names] at this
+    exact this
+  exact distance_prop this
+  have : t.length < v := by
+    simp at sat con
+    have := Trail.ud_vars twf.1 wf.1 wf.2 twf.2 (Formula.nSatCon_ud sat con)
+    simp[Trail.names] at this
+    exact this
+  exact distance_dec this
+
+
+def DPLL_moma(f : Formula)(v : Variables)(wf : f.wf ∧ v.wf f) :=
+  match f with
+  | [] => (true, [])
+  | hd::tl =>
+    let occ := occurences (hd::tl) v wf
+    internal_moma [] (hd::tl) v occ (Variables.f_cons_ne_zero wf.2 (fwf := wf.1)) wf (by simp[Trail.wf, Trail.names]) (by simp[Completenes.inv]) (by simp[occ])
