Main.lean
@@ -1,4 +1,48 @@
-import SATsolver
+import Init.System.IO
 
-def main : IO Unit :=
-  IO.println s!"Hello, {hello}!"
+import SATsolver.Experiment.Parse
+import SATsolver.Experiment.DPLL.impl
+
+def dpll_file (file: System.FilePath) : IO Nat := do
+  let (nvars, cnf) ← readDimacs file
+  let decstart ← IO.monoMsNow
+  if call : cnf.all (·.wf) then
+    if vwf : decide (Variables.wf nvars cnf) then
+    let decend ← IO.monoMsNow
+    IO.println s!"Time used: {decend-decstart}ms"
+      have wf : cnf.wf ∧ Variables.wf nvars cnf := by
+        simp at call vwf
+        have fwf := wf_check call vwf
+        exact And.intro fwf vwf
+      IO.println "start"
+      let start ← IO.monoMsNow
+      let (b, t) ← pure (DPLL_moma cnf nvars wf)
+      let stop ← IO.monoMsNow
+      IO.println s!"Time used: {stop-start}ms. Result {b} and {t}"
+      return (stop-start)
+    else
+    IO.println "Wrong amount of vars"
+    return 0
+  else
+    IO.println s!"{List.mergeSort cnf.names}"
+    IO.println "Illeagal formula"
+    return 0
+
+
+def main : IO Unit := do
+  let dir  ← System.FilePath.readDir "UUF100.430.1000"
+  let mut average := 0
+  let mut max := 0
+  let mut files := 0
+  let mut amount := 0
+  for entry in dir do
+    let time ← dpll_file entry.path
+    if time == 0 then
+      IO.println "error has been found"
+      break
+    else if max < time then max := time
+    average := time + average
+    files := files + 1
+    amount := amount + 1
+    if amount >= 20 then break
+  IO.print s!"Files run : {files}, average time {average/amount} and max time {max}"
