SATsolver/Data.lean
@@ -1,5 +1,0 @@
-/- Import Management file-/
-
-import SATsolver.Data.Clause
-import SATsolver.Data.ListTrail
-import SATsolver.Data.Formula
