SATsolver/Experiment/DPLL/Theorem.lean
@@ -247,10 +247,11 @@ theorem DPLL.all_deduced_if_con {f : Formula}{v : Variables} {wf : f.wf ∧ v.wf
 
 
 theorem DPLL.soundness {f : Formula}{v : Variables}{wf : f.wf ∧ v.wf f}{b : Bool}{t : Trail} :
-  DPLL f  v wf = (b, t) → b = true → ∃ (t : Trail), t ⊨ f := by
+  DPLL f  v wf = (b, t) → b = true → ∃ (t : Trail), t.wf ∧ t ⊨ f := by
   intro h bh
-  have := DPLL.final_state h
-  simp[bh] at this
+  have fs := DPLL.final_state h
+  have wf := DPLL.wf h
+  simp[bh] at fs
   exists t
 
 theorem DPLL.final_false {b : Bool}{f: Formula}{v : Variables}{wf : f.wf ∧ v.wf f}{t : Trail}{twf : t.wf}:
@@ -261,7 +262,7 @@ theorem DPLL.final_false {b : Bool}{f: Formula}{v : Variables}{wf : f.wf ∧ v.w
   have := Completenes.inv_completeness twf com state.2
   simp at this ⊢
   intro x xwf
-  have nohead := Completenes.from_con state.1
+  have nohead := Completenes.con_no_exist state.1
   simp at nohead
   exact this nohead x xwf
 
@@ -282,6 +283,293 @@ theorem DPLL.completeness {f : Formula}{v : Variables}{wf : f.wf ∧ v.wf f}:
   case inr rh =>
     have := DPLL.wf dplleq
     have := DPLL.final_false (twf := this) dplleq rh
+    simp at this
+    have := this t twf
+    contradiction
+
+
+theorem final_state_moma {f: Formula}{v : Variables}{occ : List (Nat × Nat)}{vz : v ≠ 0}{wf : f.wf ∧ v.wf f}{b : Bool}{t t' : Trail}{twf : t.wf ∧ ∀ n ∈ t.names, n ∈ f.names}{com : Completenes.inv t f}{hocc : occ = occurences f v wf}:
+  internal_moma t f v occ vz wf twf com hocc = (b, t') → (b = true ∧ t' ⊨ f) ∨ b = false := by
+  unfold internal_moma
+  split
+  case isTrue hsat =>
+    simp at hsat ⊢
+    intro bh heq
+    simp[←heq, hsat]
+  case isFalse hsat =>
+    split
+    case isTrue hcon =>
+      split
+      case isTrue exDec =>
+        intro h
+        exact final_state_moma h
+      case isFalse exDec =>
+        simp
+        intro bh th
+        simp[bh]
+    case isFalse hcon =>
+      simp
+      split
+      case isTrue hunit =>
+        intro h
+        exact final_state_moma h
+      case isFalse hunit =>
+        intro h
+        exact final_state_moma h
+termination_by distance t v vz
+decreasing_by
+  have : t.length < v := by
+    rename ¬decide (t⊨f) = true => sat
+    rename ¬decide (t⊭f) = true => con
+    simp at sat con
+    have := Trail.ud_vars twf.1 wf.1 wf.2 twf.2 (Formula.nSatCon_ud sat con)
+    simp[Trail.names] at this
+    exact this
+  exact distance_dec this
+  have : t.length < v := by
+    rename ¬decide (t⊨f) = true => sat
+    rename ¬decide (t⊭f) = true => con
+    simp at sat con
+    have := Trail.ud_vars twf.1 wf.1 wf.2 twf.2 (Formula.nSatCon_ud sat con)
+    simp[Trail.names] at this
+    exact this
+  exact distance_prop this
+  have : t.length ≤ v := Trail.mem_vwf twf.1 twf.2 wf.2
+  exact distance_bc this
+
+theorem DPLL_moma.final_state{f : Formula}{v : Variables}{wf : f.wf ∧ v.wf f}{b : Bool}{t : Trail}:
+DPLL_moma f  v wf = (b, t) → (b = true ∧ t ⊨ f) ∨ b = false := by
+  simp[DPLL_moma]
+  cases f
+  case nil => simp[Satisfies.sat]
+  case cons c cs =>
+    simp
+    exact final_state_moma
+
+theorem moma_wf{f: Formula}{v : Variables}{occ : List (Nat × Nat)}{vz : v ≠ 0}{wf : f.wf ∧ v.wf f}{b : Bool}{t t' : Trail}{twf : t.wf ∧ ∀ n ∈ t.names, n ∈ f.names}{com : Completenes.inv t f}{hocc : occ = occurences f v wf}:
+  internal_moma t f v occ vz wf twf com hocc = (b, t') → t'.wf := by
+  unfold internal_moma
+  split
+  case isTrue hsat =>
+    simp at hsat ⊢
+    intro bh heq
+    simp[←heq, twf.1]
+  case isFalse hsat =>
+    split
+    case isTrue hcon =>
+      split
+      case isTrue exDec =>
+        intro h
+        exact moma_wf h
+      case isFalse exDec =>
+        simp
+        intro bh th
+        simp[←th, twf.1]
+    case isFalse hcon =>
+      simp
+      split
+      case isTrue hunit =>
+        intro h
+        exact moma_wf h
+      case isFalse hunit =>
+        intro h
+        exact moma_wf h
+termination_by distance t v vz
+decreasing_by
+  have : t.length < v := by
+    rename ¬decide (t⊨f) = true => sat
+    rename ¬decide (t⊭f) = true => con
+    simp at sat con
+    have := Trail.ud_vars twf.1 wf.1 wf.2 twf.2 (Formula.nSatCon_ud sat con)
+    simp[Trail.names] at this
+    exact this
+  exact distance_dec this
+  have : t.length < v := by
+    rename ¬decide (t⊨f) = true => sat
+    rename ¬decide (t⊭f) = true => con
+    simp at sat con
+    have := Trail.ud_vars twf.1 wf.1 wf.2 twf.2 (Formula.nSatCon_ud sat con)
+    simp[Trail.names] at this
+    exact this
+  exact distance_prop this
+  have : t.length ≤ v := Trail.mem_vwf twf.1 twf.2 wf.2
+  exact distance_bc this
+
+
+theorem DPLL_moma.wf{f : Formula}{v : Variables}{wf : f.wf ∧ v.wf f}{b : Bool}{t : Trail}:
+DPLL_moma f  v wf = (b, t) → t.wf := by
+  simp[DPLL_moma]
+  cases f
+  case nil => simp; intro bh heq; simp[heq, Trail.wf, Trail.names]
+  case cons c cs =>
+    simp
+    exact moma_wf
+
+
+theorem moma_all_deduced_if_con{f: Formula}{v : Variables}{occ : List (Nat × Nat)}{vz : v ≠ 0}{wf : f.wf ∧ v.wf f}{b : Bool}{t t' : Trail}{twf : t.wf ∧ ∀ n ∈ t.names, n ∈ f.names}{com : Completenes.inv t f}{hocc : occ = occurences f v wf}:
+  internal_moma t f v occ vz wf twf com hocc = (b, t') → b = false → (t' ⊭ f ∧  ∀ a ∈ t', a.deducedP) := by
+  unfold internal_moma
+  split
+  case isTrue =>
+    simp
+    intro btrue heq bfalse
+    simp[btrue] at bfalse
+  case isFalse hsat =>
+    split
+    case isTrue hcon =>
+      split
+      case isTrue hexi => exact moma_all_deduced_if_con
+      case isFalse hexi =>
+        simp[ALit.decidedP_iff_decidedB, ←ALit.ded_iff_not_dec] at hexi
+        intro heq bfalse
+        simp at heq
+        simp[←heq.2]
+        constructor
+        case left => simpa using hcon
+        case right => exact hexi
+    case isFalse hcon =>
+      simp
+      split
+      case isTrue hunit =>
+        exact moma_all_deduced_if_con
+      case isFalse hunit =>
+        exact moma_all_deduced_if_con
+  termination_by distance t v vz
+  decreasing_by
+    have : t.length < v := by
+      rename ¬decide (t⊨f) = true => sat
+      rename ¬decide (t⊭f) = true => con
+      simp at sat con
+      have := Trail.ud_vars twf.1 wf.1 wf.2 twf.2 (Formula.nSatCon_ud sat con)
+      simp[Trail.names] at this
+      exact this
+    exact distance_dec this
+    have : t.length < v := by
+      rename ¬decide (t⊨f) = true => sat
+      rename ¬decide (t⊭f) = true => con
+      simp at sat con
+      have := Trail.ud_vars twf.1 wf.1 wf.2 twf.2 (Formula.nSatCon_ud sat con)
+      simp[Trail.names] at this
+      exact this
+    exact distance_prop this
+    have : t.length ≤ v := Trail.mem_vwf twf.1 twf.2 wf.2
+    exact distance_bc this
+
+theorem moma_com_preserved {f: Formula}{v : Variables}{occ : List (Nat × Nat)}{vz : v ≠ 0}{wf : f.wf ∧ v.wf f}{b : Bool}{t t' : Trail}{twf : t.wf ∧ ∀ n ∈ t.names, n ∈ f.names}{com : Completenes.inv t f}{hocc : occ = occurences f v wf}:
+  internal_moma t f v occ vz wf twf com hocc = (b, t') → Completenes.inv t' f := by
+  unfold internal_moma
+  split
+  case isTrue hsat =>
+    intro heq
+    simp at heq
+    rw[←heq.2]
+    exact com
+  case isFalse hsat =>
+    split
+    case isTrue hcon =>
+      split
+      case isTrue exdec=>
+        intro h
+        simp at h
+        exact moma_com_preserved h
+      case isFalse exdec =>
+        intro heq
+        simp at heq
+        rw[←heq.2]
+        exact com
+    case isFalse hcon =>
+      simp
+      split
+      case isTrue exuni =>
+        exact moma_com_preserved
+      case isFalse exuni =>
+        exact moma_com_preserved
+  termination_by distance t v vz
+  decreasing_by
+    have : t.length < v := by
+      rename ¬decide (t⊨f) = true => sat
+      rename ¬decide (t⊭f) = true => con
+      simp at sat con
+      have := Trail.ud_vars twf.1 wf.1 wf.2 twf.2 (Formula.nSatCon_ud sat con)
+      simp[Trail.names] at this
+      exact this
+    exact distance_dec this
+    have : t.length < v := by
+      rename ¬decide (t⊨f) = true => sat
+      rename ¬decide (t⊭f) = true => con
+      simp at sat con
+      have := Trail.ud_vars twf.1 wf.1 wf.2 twf.2 (Formula.nSatCon_ud sat con)
+      simp[Trail.names] at this
+      exact this
+    exact distance_prop this
+    have : t.length ≤ v := Trail.mem_vwf twf.1 twf.2 wf.2
+    exact distance_bc this
+
+theorem DPLL_moma.com_preserved {f : Formula}{v : Variables}{wf : f.wf ∧ v.wf f}{b : Bool}{t : Trail} :
+  DPLL_moma f v wf = (b, t) → Completenes.inv t f := by
+  simp[DPLL_moma]
+  cases f
+  case nil =>
+    simp
+    intro btrue heq
+    simp[heq, Completenes.inv]
+  case cons c cs =>
+    simp
+    intro h
+    exact moma_com_preserved h
+
+
+theorem DPLL_moma.all_deduced_if_con {f : Formula}{v : Variables} {wf : f.wf ∧ v.wf f}{b : Bool}{t : Trail} :
+  DPLL_moma f v wf = (b, t) → b = false → t ⊭ f ∧ ∀ a ∈ t, a.deducedP := by
+  simp[DPLL_moma]
+  cases f
+  case nil =>
+    simp
+    intro btrue hnil bfalse
+    simp[btrue] at bfalse
+  case cons x xs =>
+    simp
+    intro heq bfalse
+    exact moma_all_deduced_if_con heq bfalse
+
+
+theorem DPLL_moma.soundness {f : Formula}{v : Variables}{wf : f.wf ∧ v.wf f}{b : Bool}{t : Trail} :
+  DPLL_moma f  v wf = (b, t) → b = true → ∃ (t : Trail), t.wf ∧ t ⊨ f := by
+  intro h bh
+  have fs := DPLL_moma.final_state h
+  have wf := DPLL_moma.wf h
+  simp[bh] at fs
+  exists t
+
+theorem DPLL_moma.final_false {b : Bool}{f: Formula}{v : Variables}{wf : f.wf ∧ v.wf f}{t : Trail}{twf : t.wf}:
+  DPLL_moma f v wf = (b, t) → b = false → ¬ (∃ (t : Trail), t.wf ∧ t ⊨ f) := by
+  intro heq bfalse
+  have state := DPLL_moma.all_deduced_if_con heq bfalse
+  have com := DPLL_moma.com_preserved heq
+  have := Completenes.inv_completeness twf com state.2
+  simp at this ⊢
+  intro x xwf
+  have nohead := Completenes.con_no_exist state.1
+  simp at nohead
+  exact this nohead x xwf
+
+
+theorem DPLL_moma.completeness {f : Formula}{v : Variables}{wf : f.wf ∧ v.wf f}:
+  (∃ (t : Trail), t.wf ∧ t ⊨ f) → ∃ (t : Trail), DPLL_moma f v wf = (true, t) := by
+  intro h
+  obtain ⟨ t, twf, tsat ⟩ := h
+  let dpll : (Bool ×  Trail) := DPLL_moma f v wf
+  let b := dpll.1
+  let t' := dpll.2
+  have dplleq : DPLL_moma f v wf = (b, t') := by simp[dpll, b ,t']
+  have := DPLL_moma.final_state dplleq
+  cases this
+  case inl lh =>
+    exists t'
+    rw[dplleq, lh.1]
+  case inr rh =>
+    have := DPLL_moma.wf dplleq
+    have := DPLL_moma.final_false (twf := this) dplleq rh
     simp at this
     have := this t twf
     contradiction
