SATsolver/Experiment/Parse.lean
@@ -1,52 +1,49 @@
-import SatProver.CNF
+import SATsolver.Experiment.Data.Formula
 
-partial def readLines (filename : System.FilePath) : IO (List String) := do
-  let handle ← IO.FS.Handle.mk filename IO.FS.Mode.read
-  let rec loop (lines : List String) : IO (List String) := do
-    let line ← handle.getLine
-    if line.isEmpty ∨ line.startsWith "%" then
-      pure lines.reverse
-    else if line.startsWith "c" then
-      loop lines
-    else
-      let cleaned := line.trim
-      loop (cleaned :: lines)
-  loop []
+open IO
 
 def parseClause (line : String) : Clause :=
-  (
-    line.splitOn " "
-    |>.filter (· ≠ "")
-    |>.map (String.toInt!)
-    |>.takeWhile (· ≠ 0)
-  ).toArray
+  line.splitOn " "
+  |>.foldl
+      (fun acc tok =>
+        if tok.isEmpty then acc
+        else
+          let i := String.toInt! tok
+          if i == 0 then acc
+          else
+            let lit :=
+              if i < 0 then
+                Lit.neg (Int.natAbs i)
+              else
+                Lit.pos (Int.natAbs i)
+            lit :: acc)
+      []
+  |> List.reverse
 
-def parseDimacs (lines : List String) : Except String CNF := do
-  let mut nVars: Nat := 0
-  let mut nClauses: Nat := 0
-  let mut clauses : Array Clause := #[]
-  for line in lines do
-    if line.startsWith "c" ∨ line.startsWith "%" then
-      pure ()
-    else if line.startsWith "p" then
-      let vals := line.splitOn " "
-      if vals.length ≠ 4 then
-        throw "Invalid file. Header wrong length"
+def readDimacs (fileName : System.FilePath) : IO (Nat × Formula) := do
+  IO.FS.withFile fileName .read fun h => do
+    let mut nVars : Nat := 0
+    let mut clauses : Formula := []
+
+    while true do
+      let line ← h.getLine
+      if line.isEmpty then
+        break
+
+      let line := line.trim
+      if line.isEmpty ∨ line.startsWith "c" then
+        continue
+
+      if line.startsWith "p" then
+        let parts := line.splitOn " " |>.filter (· ≠ "")
+        if parts.length ≠ 4 then
+          throw <| IO.userError "Invalid DIMACS header"
+        nVars := parts[2]!.toNat!
+      else if line.startsWith "%" then
+        break
       else
-        nVars := vals[2]!.toNat!
-        nClauses := vals[3]!.toNat!
-    else
-      let clause := parseClause line
-      if ¬clause.isEmpty then
-        clauses := clauses ++ [parseClause line]
-  return ⟨ nVars, nClauses, clauses ⟩
+        let clause := parseClause line
+        if ¬ clause.isEmpty then
+          clauses := clause :: clauses
 
-def readDimacs (fileName : System.FilePath) : IO CNF := do
-  let lines ←  readLines fileName
-  match parseDimacs lines with
-    | .ok cnf => pure cnf
-    | .error msg => throw <| IO.userError msg
-
-def main : IO Unit := do
-  let cnf ← readDimacs "test.cnf"
-  IO.println cnf
+    return (nVars, clauses.reverse)
