SATsolver/SolverState.lean
@@ -1,9 +1,0 @@
-import SATsolver.Data.Trail
-import SATsolver.Data.Formula
-
-structure State where
-  M : Trail
-  N : Formula
-  U : Formula
-  k : Nat
-  C : Formula
